theories/examples/simple.v
@@ -1,7 +1,7 @@
 From iris.proofmode Require Import tactics.
 (* From iris.program_logic Require Export weakestpre. *)
 From self.lang Require Export notation primitive_laws lang class_instances proofmode.
-From self Require Import dProp view lang.
+From self Require Import dprop view lang.
 From self Require Export weakestpre.
 
 Definition prog : expr := let: "l" := ref #1 in ! "l".
@@ -12,10 +12,11 @@ Definition pure : expr :=
   "a" + "b".
 
 Section specs.
-  Context `{!nvmG Σ}.
+  Context `{!nvmG Σ, !wpnvmG Σ}.
 
   Lemma wp_bin_op : ⊢ WP (#1 + #2) {{ v, True }}.
   Proof.
+    wp_pure _.
     wp_pures.
     done.
   Qed.
