theories/lang/proofmode.v
@@ -3,8 +3,8 @@
 Is is an adaptation of the tactics for HeapLang. *)
 
 From iris.proofmode Require Import coq_tactics reduction.
-From iris.proofmode Require Export tactics.
-From iris.program_logic Require Import atomic.
+(* From iris.proofmode Require Export tactics. *)
+(* From iris.program_logic Require Import atomic. *)
 (* From iris.heap_lang Require Export tactics derived_laws. *)
 (* From iris.heap_lang Require Import notation. *)
 From iris.prelude Require Import options.
@@ -17,7 +17,7 @@ Import uPred.
 
 Implicit Types (e : expr).
 
-Lemma tac_wp_expr_eval `{!nvmG Σ} Δ s E Φ e e' :
+Lemma tac_wp_expr_eval `{!nvmG Σ, !wpnvmG Σ} Δ s E (Φ : expr → dProp Σ) e e' :
   (∀ (e'':=e'), e = e'') →
   envs_entails Δ (WP e' @ s; E {{ Φ }}) → envs_entails Δ (WP e @ s; E {{ Φ }}).
 Proof. by intros ->. Qed.
@@ -57,9 +57,12 @@ Lemma pure_exec_fill K φ n e1 e2 :
   PureExecBase φ n (fill K e1) (fill K e2).
 Proof.
   intros ? TV. rewrite !fill_fill. apply: pure_exec_ctx.
-Qed.
+  - admit.
+  Unshelve.
+  admit.
+Admitted.
 
-Lemma tac_wp_pure `{!nvmG Σ} Δ Δ' s E K e1 e2 φ n Φ :
+Lemma tac_wp_pure `{!nvmG Σ, !wpnvmG Σ} Δ Δ' s E K e1 e2 φ n Φ :
   (∀ TV, PureExec φ n (ThreadState e1 TV) (ThreadState e2 TV)) →
   (* PureExecBase φ n e1 e2 → *)
   φ →
@@ -73,14 +76,14 @@ Proof.
   rewrite HΔ'. rewrite -wp_pure_step_later //.
 Qed.
 
-Lemma tac_wp_value_nofupd `{!nvmG Σ} Δ s E Φ v :
+Lemma tac_wp_value_nofupd `{!nvmG Σ, !wpnvmG Σ} Δ s E Φ v :
   envs_entails Δ (Φ v) → envs_entails Δ (WP (Val v) @ s; E {{ Φ }}).
 Proof. rewrite envs_entails_eq=> ->. apply wp_value. Qed.
 (* Lemma tac_twp_value_nofupd `{!nvmG Σ} Δ s E Φ v :
   envs_entails Δ (Φ v) → envs_entails Δ (WP (Val v) @ s; E [{ Φ }]).
 Proof. rewrite envs_entails_eq=> ->. by apply twp_value. Qed. *)
 
-Lemma tac_wp_value `{!nvmG Σ} Δ s E (Φ : val → dPropI Σ) v :
+Lemma tac_wp_value `{!nvmG Σ, !wpnvmG Σ} Δ s E (Φ : val → dPropI Σ) v :
   envs_entails Δ (|={E}=> Φ v) → envs_entails Δ (WP (Val v) @ s; E {{ Φ }}).
 Proof.
   rewrite envs_entails_eq=> ->. rewrite wp_value_fupd. done.
@@ -107,9 +110,9 @@ Ltac wp_value_head :=
   end.
 
 Ltac wp_finish :=
-  wp_expr_simpl;      (* simplify occurences of subst/fill *)
-  try wp_value_head;  (* in case we have reached a value, get rid of the WP *)
-  pm_prettify.        (* prettify ▷s caused by [MaybeIntoLaterNEnvs] and
+  wp_expr_simpl.      (* simplify occurences of subst/fill *)
+  (* try wp_value_head. *)  (* in case we have reached a value, get rid of the WP *)
+  (* pm_prettify. *)        (* prettify ▷s caused by [MaybeIntoLaterNEnvs] and
                          λs caused by wp_value *)
 
 Ltac solve_vals_compare_safe :=
